examples/steel/arraystructs/Steel.C.Frac.fst
@@ -1,6 +1,5 @@
 module Steel.C.Frac
 
-open FStar.PCM
 open Steel.C.PCM
 open Steel.C.Ref
 open Steel.Effect
